rustexamples/test/48_shr_ref_invariant.rs
@@ -1,0 +1,22 @@
+struct A<'a>{
+    x: &'a mut i32,
+    y: &'a i32
+}
+
+fn use_shr_ref<'b>(r: &'b i32) {
+    let mut tmp: i32 = *r;
+}
+
+// rustc +nightly 48_shr_ref_invariant.rs -Z polonius=next
+
+fn main(){
+    let mut v1: i32 = 1;
+    let mut v2: i32 = 2;
+    let mut v3: i32 = 3;
+    let mut a: A = A {x: &mut v1, y: &v2};
+    let mut p: & &i32 = &a.y; // We generate 'a = 'p2 but Polonius would generate 'a : 'p2
+    a.x = &mut v3; // 'p2 contains v3 because we change 'a which also changes 'p2 since 'p2 = 'a. It is an imprecision introduced by invariant w.r.t. 'p2
+    v3 = 4; // error occurs here because we restrict 'p2 is invariant of 'a. This error does not occur in Polonius becasue the subset relation ['a:'p2] is not flowed here so loan [v3] is not flowed into 'p2 at this point. But this error occurs in NLL because 'a : 'p2 is not cleared even if 'a is dead?
+    use_shr_ref(*p);
+    // use_shr_ref(a.y); //'a is still live here. If we uncomment this line and comment the last line, there would be error in Polonius borrow checker because loan [v3] is flowed to 'p2. However, using a.y should be irrlevant to the loan [v3]. But since we use 'a to abstract both regions of a.x and a.y, we have this imprecision here.
+}
